src/smtencoding/FStarC.SMTEncoding.Util.fst
@@ -83,9 +83,13 @@ let mkBvUlt = norng mkBvUlt
 let mkBvUext sz = norng (mkBvUext sz)
 let mkBvToNat = norng mkBvToNat
 let mkITE = norng mkITE
+let mkCases = norng mkCases
+
 let mkStrLen = norng mkStrLen
 let mkStrCat = norng mkStrCat
-let mkCases = norng mkCases
+let mkStrSubStr = norng mkStrSubStr
+let mkStrAt = norng mkStrAt
+let mkStrIndexOf = norng mkStrIndexOf
 
 let norng2 f = fun x y -> f x y Range.dummyRange
 let norng3 f = fun x y z -> f x y z Range.dummyRange
